\documentclass[11pt]{amsart}
\usepackage{geometry}                % See geometry.pdf to learn the layout options. There are lots.
\geometry{letterpaper}                   % ... or a4paper or a5paper or ... 
\input{../p.tex}
\title{Approximating the Optimal State Abstraction}
\author{}
\date{}                                           % Activate to display a given date or no date

% --- Note Commands ---
\newcommand\davenote[1]{\textcolor{blue}{Dave: #1}}

\begin{document}
\maketitle
\section{Results}

Recall, there is a ground MDP $M$ we want to solve. We homogenize to an MDP $M'$, and apply $\phi$ to $M'$ to get an abstract MDP $A$.

For each approximate $\phi$ type, we want to show, $\forall_{\epsilon} : \epsilon \in [0 : \infty)$
\begin{equation}
\forall_{s,a} : | V^{\pi^*_M}(s) - V^{\pi^*_{M'}}(s) | \leq \epsilon
\end{equation}

We consider four $\phi$ types:
% phi model
\begin{align*}
\encircle{\text{ $\phi_m$ }}\ & : \phi_{m}(s_1) = \phi_m(s_2) \rightarrow \forall_a |\mathcal{R}(s_1,a) - \mathcal{R}(s_2,a)| \leq \epsilon \ \wedge\ 
\forall_{a,s' \in \phi^{-1}(\bar{s})} | \mathcal{T}(s_1,a,s') - \mathcal{T}(s_2,a,s') | \leq \epsilon \\
\encircle{\text{ $\phi_{Q^*}$ }}\ & : \phi_{Q^*}(s_1) = \phi_{Q^*}(s_2) \rightarrow \forall_a |Q^*(s_1,a) - Q^*(s_2,a)| \leq \epsilon \\
\encircle{\text{ $\phi_{D}$ }}\ & : \phi_D(s_1) = \phi_D(s_2) \rightarrow \Delta \left( \Pr_{a \in \mathcal{A}}(a \mid s_1) \mid\mid \Pr_{a \in \mathcal{A}}(a \mid s_2) \right) \leq \epsilon \\
\encircle{\text{ $\phi_{a^*}$ }}\ & : \phi_{a^*}(s_1) = \phi_{a^*}(s_2) \rightarrow \argmax_a Q^*(s_1,a) = \argmax_a Q^*(s_2, a) \wedge |\max_a Q^*(s_1,a) - \max_a Q^*(s_2,a)| \leq \epsilon  \\
\end{align*}

\elem{NOTE:} Instead of performing the abstraction w.r.t. $\phi$, our new strategy is to, given an MDP $M$ (and possibly some other information, $\kappa$), apply a function $H$ to create $M'$, for which all of the old $\phi$ functions may operate.

Specifically:
\begin{multline}
H(f, \epsilon) \rightarrow f' \text{  s.t.  } \\ \forall_{(s_1,a,s_1'),(s_2,a,s_2')} \left(f'(s_1,a,s_1') = f'(s_2,a,s_2') \rightarrow | f(s_1,a,s_1') - f(s_2,a,s_2') | \leq \epsilon\right)
\end{multline}

Where:
\begin{equation}
f(s,a,s') \rightarrow \mathbb{R}
\end{equation}

% Other results to consider: phi compression can be arbitrarily bad for other methods of approximate compression. Sample complexity increase can be arbitrarily large.

\elem{NOTE:} We are {\it not} going to provide results for $\phi_{\pi^*}$, since relaxing equality of optimal actions doesn't mean anything.

\elem{NOTE:} Additionally, we are {\it not} going to provide results for $\phi_{Q^\pi}$, since as Lihong's paper notes, ``It is an open question how to find $Q^\pi$ irrelevance abstractions without enumerating all possible policies, they do not give results. Furthermore, an MDP for which this is true is an awfully weird MDP...

\elem{NOTE:} For $\phi_D$, we consider the space of distributions on optimal Q values where:
\begin{equation}
f(Q(s,a)) > f(Q(s,a_2)) \rightarrow Q(s,a_1) > Q(s,a_2)
\end{equation}

\newpage
% Subsection: phi_m Results
\section{$\phi_{m}$ Results}

Let the maximum upper bound between optimal behavior in the noisy and ground MDP be called $B_s$.

\begin{align*}
B_{s} &= \max_{s,a}|Q'(s,a)-Q(s,a)|\\
B_{s} &= \max_{s,a}|R'(s,a) - R(s,a) + \gamma \sum_{s'}\left[T'(s,a,s')\max_{a'}Q'(s',a')-T(s,a,s')\max_{a'}Q(s', a')\right]|\\
&\forall s' \text{ WLOG } T'(s,a,s')\max_{a'}Q'(s',a') \geq T(s,a,s')\max_{a'}Q(s',a')\\
&\text{Applying max is a non-expansion}\\
&=\max_{s,a}(|R'(s,a)-R(s,a)| + \gamma \sum_{s'} \max_{a'} \left[(T(s,a,s')+T'(s,a,s')-T(s,a,s'))Q'(s', a')-T(s,a,s')Q(s',a')\right])\\
\\
&\leq \max_{s,a}|R'_s-R_s|+\max_{s,a}\gamma \sum_{s'} \max_{a'} \left[(T(s,a,s')+\epsilon_{\text{transition}})Q'(s',a') - T(s,a,s')Q(s',a')\right]\\
&\leq \epsilon_{\text{reward}}+\max_{s,a}\gamma \sum_{s'} \max_{a'} \left[(T(s,a,s')Q'(s',a')+\epsilon_{\text{transition}}Q'(s',a') - T(s,a,s')Q(s',a')\right]\\
\\
&\leq \epsilon_{\text{reward}} + \max_{s,a} \gamma \sum_{s'} \max_{a'} \left[(T(s,a,s')(Q'(s',a')-Q(s',a'))+\epsilon_{\text{transition}}Q'(s',a') \right]\\
&\leq \epsilon_{\text{reward}}+\gamma |\mathcal{S}|\epsilon_{transition}Q'_{\text{max}} + \gamma \sum_{s'}\left[ T(s,a,s') B_s\right]\\
&\leq \epsilon_{\text{reward}} + \gamma B_{s} + \gamma |\mathcal{S}|\epsilon_{\text{transition}}Q'_{max}\\
&\text{Applying }Q'_{max}=V'_{max} \leq V_{max}=\frac{1}{1-\gamma}\\
B_{s} &\leq 
\frac
{{\epsilon_{\text{reward}}} + \gamma |\mathcal{S}|\epsilon_{transition}}
{(1-\gamma)^2}
\end{align*}

Therefore:
\begin{equation}
\forall_{s,a} : |Q'(s,a) - Q(s,a)| \leq \max_{s,a}|Q'(s,a)-Q(s,a)| \leq  \frac{{\epsilon_{\text{reward}}} + \gamma |\mathcal{S}|\epsilon_{transition} }{(1-\gamma)^2}
\end{equation}

Consequently, from the below $\phi_Q^*$ results, we conclude that:
\begin{equation}
\forall_s : |V^{\pi^*_M}(s) - V^{\pi^*_{M'}}(s)| \leq \frac{{\epsilon_{\text{reward}}} + \gamma |\mathcal{S}|\epsilon_{transition}}{(1-\gamma)^3}
\end{equation}
\qed


\newpage
% Subsection: phi_Q^* Results
\section{$\phi_{Q^*}$ Results}

We consider a non-temporally homogenized MDP parameterized by T, such that for the first T time steps the MDP is defined as the abstract MDP, and after T time steps, the MDP becomes identical to the ground MDP.

We proceed by induction on T.

\elem{Base:}

When T = 0, we show that:
\begin{equation}
|V^{\pi_G^S}(s) - V_0(s)| \leq \epsilon
\end{equation}

Trivial, since $V_0 = V^{\pi_G^S}(s)$.

\elem{Inductive:}

IH: Suppose $|V^{\pi_G^*}(s) - V_T(s)| \leq \sum_{t=o}^T \epsilon \gamma^t$.

WTS: $|V^{\pi_G^*}(s) - V_{T+1}(s)| \leq \sum_{t=o}^{T+1} \epsilon \gamma^t$.

\begin{align*}
V_{T+1}(s) &= \max_a \left[R_{T+1}(s,a) + \gamma \sum_s' T_{T+1}(s,a,s')V_T(s')\right] \\
&\leq \max_a \left[R_{T+1}(s,a) + \gamma \sum_s' T_{T+1}(s,a,s')\left(V_0(s) + \sum_{t=0}^T\epsilon\gamma^t \right) \right] \\
&= \gamma\left(\sum_{t=0}^T\epsilon\gamma^T\right) + \max_a \left[R_{T+1}(s,a) + \gamma \sum_s' T_{T+1}(s,a,s')V_0(s') \right] \\
&= \gamma\left(\sum_{t=0}^T\epsilon\gamma^T\right) + \max_a \left[\sum_{g \in s} R_{G}(g,a)\omega(g) + \gamma \sum_s' \sum_{g \in s}T_G(g,a,s')\omega(g)V_0(s') \right] \\
&= \gamma\left(\sum_{t=0}^T\epsilon\gamma^T\right) + \epsilon + \left(\max_a Q_G(s,a)\right) \\
&= \sum_{t=0}^{T+1} \epsilon \gamma^{T+1} + \max_a Q^{\pi_G^*}(s,a) \\
&= \frac{\epsilon}{1-\gamma} + V^{\pi_G^*}(s) \\
\end{align*}
\begin{equation}
\therefore |V^{\pi_G^*}(s) - V_{T+1}(s)| \leq | V^{\pi_G^*}(s) - \frac{\epsilon}{1-\gamma} + V^{\pi_G^*}(s)| = \frac{\epsilon}{1-\gamma} \qed
\end{equation}

%We know:
%\begin{equation}
%\forall_{s_1,s_2,a} : \phi_{Q^*}(s_1) = \phi_{Q^*}(s_2) \rightarrow | Q^{\pi^*_M}(s_1,a) - Q^{\pi^*_{M}}(s_2,a)| \leq \epsilon
%\label{eq:phi_q_assumption}
%\end{equation}
%
%Since `max' is a non-expansion, we know:
%\begin{equation}
%\forall_s : |\max_a Q^{\pi^*_M}(s,a) - \max_{a'} Q^{\pi^*_{M'}}(s,a')| \leq \max_b | Q^{\pi^*_M}(s,b) - Q^{\pi^*_{M'}}(s,b)|
%\end{equation}
%
%From Equation~\ref{eq:phi_q_assumption}, we know:
%\begin{equation}
%\forall_s : |\max_a Q^{\pi^*_M}(s,a) - \max_{a'} Q^{\pi^*_{M'}}(s,a')| \leq \max_b | Q^{\pi^*_M}(s,b) - Q^{\pi^*_{M'}}(s,b)| \leq \epsilon
%\end{equation}
%
%But since $\forall_\pi : V^{\pi} = \max_a Q^\pi(s,a)$, we conclude:
%\begin{equation}
%\forall_s : |V^{\pi^*_M}(s) - V^{\pi^*_{M'}}(s)| \leq \epsilon
%\end{equation}
%\qed

\newpage
% Subsection: phi_Mult Results
\section{$\phi_{Mult}$ Results}

\begin{equation}
\forall_{s_1, s_2 \in \mathcal{S}_G} : \phi_{Mult}(s_1) = \phi_{Mult}(s_2) \rightarrow \forall_{i \in [0:|\mathcal{A}| - 1]} | g(s_1, a_i) - g(s_2, a_i) | \leq \epsilon
\label{eq:phi_d}
\end{equation}

Where:
\begin{equation}
g(s,a) = \frac{Q(s,a)}{\sum_j Q(s,a_j)}
\end{equation}

And:
\begin{equation}
|\sum_j Q(s_1,a_j) - Q(s_2,a_j) | \leq k\epsilon
\end{equation}

So:
\begin{equation}
\forall_{s_1,s_2} \forall_a : | \frac{Q(s_1,a)}{\sum_j Q(s_1,a_j)} - \frac{Q(s_2,a)}{\sum_j Q(s_2,a_j)} | \leq \epsilon
\end{equation}

Let:
\begin{align}
Q_1 &= Q(s_1,a) &Q_2 &= Q(s_2,a) \\
D_1 &= \sum_j Q(s_1,a_j) &D_2 &= \sum_j Q(s_2,a_j) 
\end{align}

So:
\begin{equation}
\forall_{s_1,s_2} \forall_a : | \frac{Q(s_1,a)}{D_1} - \frac{Q(s_2,a)}{D_2} | \leq \epsilon
\end{equation}

Therefore:
\begin{align*}
-\epsilon \leq \frac{Q_1}{D_1} - \frac{Q_1}{D_2} \leq \epsilon \\
-\epsilon \leq \frac{Q_1}{D_1} - \frac{Q_1}{D_1 \pm k\epsilon} \leq \epsilon \\
\end{align*}

% Plus Case
\encircle{+}
\begin{align*}
-\epsilon &\leq \frac{Q_1}{D_1} - \frac{Q_1}{D_1 \pm k\epsilon} \leq \epsilon \\
-\epsilon &\leq \frac{Q_1 D_1 + Q_1 k \epsilon - Q_2 D_1}{D_1^2 + D_1 k \epsilon} \leq \epsilon \\
-\epsilon &\leq \frac{D_1 (Q_1 + \frac{Q_1 k \epsilon}{D_1} - Q_2)}{D_1 (D_1 + k \epsilon)} \leq \epsilon \\
-\epsilon &\leq \frac{Q_1 + \frac{Q_1 k \epsilon}{D_1} - Q_2}{D_1 + k \epsilon} \leq \epsilon \\
-\epsilon*(D_1 + k \epsilon) &\leq Q_1 + \frac{Q_1 k \epsilon}{D_1} - Q_2 \leq \epsilon*(D_1 + k \epsilon) \\
\end{align*}

Let: $A = \frac{Q_1 k \epsilon}{D_1}$:
\begin{align*}
-\epsilon*(D_1 + k \epsilon) - A &\leq Q_1 - Q_2 \leq \epsilon*(D_1 + k \epsilon) - A \\
-\epsilon D_1 - k \epsilon^2 - A &\leq Q_1 - Q_2 \leq \epsilon D_1 + k \epsilon^2 - A \\
-\epsilon D_1 - k \epsilon^2 - A &\leq Q_1 - Q_2 \leq \epsilon D_1 + k \epsilon^2
\end{align*}


% Minus Case
\encircle{-}
\begin{align*}
-\epsilon &\leq \frac{Q_1}{D_1} - \frac{Q_1}{D_1 \pm k\epsilon} \leq \epsilon \\
-\epsilon &\leq \frac{Q_1 D_1 - Q_1 k \epsilon - Q_2 D_1}{D_1^2 - D_1 k \epsilon} \leq \epsilon \\
-\epsilon &\leq \frac{D_1 (Q_1 - \frac{Q_1 k \epsilon}{D_1} - Q_2)}{D_1 (D_1 - k \epsilon)} \leq \epsilon \\
-\epsilon &\leq \frac{Q_1 - \frac{Q_1 k \epsilon}{D_1} - Q_2}{D_1 - k \epsilon} \leq \epsilon \\
-\epsilon*(D_1 - k \epsilon) &\leq Q_1 - \frac{Q_1 k \epsilon}{D_1} - Q_2 \leq \epsilon*(D_1 - k \epsilon) \\
\end{align*}

Let: $A = \frac{Q_1 k \epsilon}{D_1}$:
\begin{align*}
-\epsilon*(D_1 - k \epsilon) + A &\leq Q_1 - Q_2 \leq \epsilon*(D_1 - k \epsilon) + A \\
-\epsilon D_1 + k \epsilon^2 + A &\leq Q_1 - Q_2 \leq \epsilon D_1 - k \epsilon^2 + A \\
-\epsilon D_1 + k \epsilon^2 + A &\leq Q_1 - Q_2 \leq \epsilon D_1 - k \epsilon^2 + A
\end{align*}

\begin{equation}
\therefore |Q_1 - Q_2| \leq \epsilon D_1 + k \epsilon^2 + A \qed
\end{equation}

\newpage
\thm{Theorem}{1}{There are three pairs of functions, $\langle \phi_1, f_1 \rangle$, $\langle \phi_2, f_2 \rangle$, and $\langle \phi_3, f_3 \rangle$ such that:
\begin{equation*}
\forall_{s_1, s_2 \in S_M} : \phi_{i}(s_1) = \phi_{i}(s_2) \rightarrow \forall_a :  |f_i(s_1,a) - f_i(s_2,a)| \leq \epsilon
\end{equation*}

Where, the MDP resulting from the abstracted state space, $A$, when solved, provides the policy $\pi^*_A$, such that:
\begin{equation*}
\forall_{s \in S_M} : | V^{\pi^*_M}(s) - V^{\pi^*_{A}}(s) | \leq poly(\epsilon)
\end{equation*}}

\newpage
% Subsection: phi_a^* Results
\section{$\phi_{a^*}$ Results}




% --- BIBLIOGRAPHY ---
\newpage
\bibliography{sca_bib}

\end{document}
